LeanProjeto2/StarLanguage/Axioms2.lean
@@ -6,6 +6,11 @@
 import LeanProjeto2.FOLanguage
 import LeanProjeto2.StarLanguage.FiniteTypes
 import LeanProjeto2.StarLanguage.Syntax
+import Init.Data.List.Basic
+import Init.Data.List.Lemmas
+import Mathlib.Data.Finset.Basic
+import Mathlib.Data.Multiset.Basic
+import Batteries
 import MathLib.Tactic
 
 open FOLang
@@ -13,6 +18,7 @@ open LFormula
 open Term
 open Formula
 open Set
+open Batteries
 
 -- --------------------------------------
 -- --------------------------------------
@@ -23,23 +29,188 @@ open Set
 
 namespace Axioms
 
-def AxiomE1 (t:Term) : Formula :=                                    t=₁t
-def AxiomE2 (t₁ t₂ :Term) (A : Formula) (hA : isBase A) : Formula := (t₁=₁t₂) ∧₁ (A →₁ A)     -- TBD: falta substituição aqui
-def AxiomU (x : String) (t : Term) (A : Formula) : Formula :=        (b∀₁₁ x t A) ↔₁ (∀₁₁ x (((var x) ∈₁ t) →₁ A))
-def AxiomC1 (t₁ t₂ : Term) : Formula :=                              ((Π₁·t₁)·t₂) =₁ t₁
-def AxiomC2 (t₁ t₂ t₃ : Term) : Formula :=                           (((Σ₁·t₁)·t₂)·t₃) =₁ ((t₁·t₃)·(t₂·t₃))
-def AxiomP1 (t₁ t₂ : Term) : Formula :=                              ((ind_⋃₁·(𝔰₁·t₁))·t₂) =₁ (t₂·t₁)
-def AxiomP2 (t₁ t₂ t₃ : Term) : Formula :=                           ((ind_⋃₁·((∪₁·t₁)·t₂))·t₃) =₁ ((∪₁·((ind_⋃₁·t₁)·t₃))·((ind_⋃₁·t₂)·t₃))
-def AxiomS1 (t₁ t₂ : Term) : Formula :=                              (t₁ ∈₁ (𝔰₁·t₂)) ↔₁ (t₁ =₁ t₂)
-def AxiomS2 (t₁ t₂ t₃ : Term) : Formula :=                           (t₁ ∈₁ ((∪₁·t₂)·t₃) ) ↔₁ ((t₁ ∈₁ t₂) ∨₁ (t₁ ∈₁ t₃))
-def AxiomS3 (a f b : Term) (x : String) : Formula :=                 (b ∈₁ ((ind_⋃₁·a)·f)) ↔₁ (b∃₁₁ x a (b ∈₁ (f·(var x))))
--- TBD: FALTA AXS4
+def axiomE1 (x : String) : Formula :=
+  (var x)=₁(var x)
+def axiomE2 (x₁ x₂ : String) (A : Formula) (hA : isBase A) : Formula :=
+  (((var x₁)=₁(var x₂)) ∧₁ A) →₁ (A.subst (HashMap.ofList ([x₁].zip ([x₂].tt))))
+def axiomUn (x : String) (t : String) (A : Formula) : Formula :=
+  (b∀₁₁ x (var t) A) ↔₁ (∀₁₁ x (((var x) ∈₁ (var t)) →₁ A))
+def axiomC1 (x₁ x₂ : String) : Formula :=
+  ((Π₁·(var x₁))·(var x₂)) =₁ (var x₁)
+def axiomC2 (x₁ x₂ x₃ : String) : Formula :=
+  (((Σ₁·(var x₁))·(var x₂))·(var x₃)) =₁ (((var x₁)·(var x₃))·((var x₂)·(var x₃)))
+def axiomP1 (x₁ x₂ : String) : Formula :=
+  ((ind_⋃₁·(𝔰₁·(var x₁)))·(var x₂)) =₁ ((var x₂)·(var x₁))
+def axiomP2 (x₁ x₂ x₃ : String) : Formula :=
+  ((ind_⋃₁·((∪₁·(var x₁))·(var x₂)))·(var x₃)) =₁ ((∪₁·((ind_⋃₁·(var x₁))·(var x₃)))·((ind_⋃₁·(var x₂))·(var x₃)))
+def axiomS1 (x₁ x₂ : String) : Formula :=
+  ((var x₁) ∈₁ (𝔰₁·(var x₂))) ↔₁ ((var x₁) =₁ (var x₂))
+def axiomS2 (x₁ x₂ x₃ : String) : Formula :=
+  ((var x₁) ∈₁ ((∪₁·(var x₂))·(var x₃)) ) ↔₁ (((var x₁) ∈₁ (var x₂)) ∨₁ ((var x₁) ∈₁ (var x₃)))
+def axiomS3 (b a f x : String) : Formula :=
+  ((var b) ∈₁ ((ind_⋃₁·(var a))·(var f))) ↔₁ (b∃₁₁ x (var a) ((var b) ∈₁ ((var f)·(var x))))
+def axiomS4 (x₁ x₂ : String) : Formula :=
+  b∃₁₁ x₂ (var x₁) ((var x₂) ∈₁ (var x₁))
+
+
+-- LEMMA: substituir não altera baseness
+lemma Subst_isBase (A : Formula) (hA : isBase A) (x : List String) (t : List Term) : isBase (A.subst (HashMap.ofList (x.zip t))) := by
+  cases hA
+  . rename_i isAt_A
+    sorry
+  . rename_i A isB_A
+    sorry
+  . rename_i A B isB_A isB_B
+    sorry
+  . rename_i A x' t' isB_A
+    sorry
+
+
+/-
+LEMAS: A MAIORIA DOS AXIOMAS SÃO UNIV CLOSURES DE BASE FORMULAS
+-/
+
+open Formula
+open isAtomic
+open isBase
+
+lemma AxiomE1_univ_of_base : (isBase (axiomE1 x)) := by
+  unfold axiomE1
+  exact b_atom (isAtomic.at_eq (var x) (var x))
+
+lemma AxiomE2_univ_of_base : (isBase (axiomE2 x₁ x₂ A hA)) := by
+  unfold axiomE2
+  have H1 := Subst_isBase A hA [x₁] [x₂].tt
+  have H2 := b_atom (isAtomic.at_eq (var x₁) (var x₂))
+  have H3 := Conj_base ((var x₁)=₁(var x₂)) A H2 hA
+  exact Imp_base ((var x₁=₁var x₂)∧₁A) (A.subst (HashMap.ofList ([x₁].zip [x₂].tt))) H3 H1
+
+-- COMMENT: AxiomUn_univ_of_base não dá porque axiomUn não é base :)
+
+lemma AxiomC1_univ_of_base : (isBase (axiomC1 x₁ x₂)) := by
+  unfold axiomC1
+  exact b_atom (isAtomic.at_eq ((Π₁·var x₁)·var x₂) (var x₁))
+
+lemma AxiomC2_univ_of_base : (isBase (axiomC2 x₁ x₂ x₃)) := by
+  unfold axiomC2
+  exact b_atom (isAtomic.at_eq (((Σ₁·(var x₁))·(var x₂))·(var x₃)) (((var x₁)·(var x₃))·((var x₂)·(var x₃))))
+
+lemma AxiomP1_univ_of_base : (isBase (axiomP1 x₁ x₂)) := by
+  unfold axiomP1
+  exact b_atom (isAtomic.at_eq ((ind_⋃₁·(𝔰₁·(var x₁)))·(var x₂)) ((var x₂)·(var x₁)))
+
+lemma AxiomP2_univ_of_base : (isBase (axiomP2 x₁ x₂ x₃)) := by
+  unfold axiomP2
+  exact b_atom (isAtomic.at_eq ((ind_⋃₁·((∪₁·(var x₁))·(var x₂)))·(var x₃)) ((∪₁·((ind_⋃₁·(var x₁))·(var x₃)))·((ind_⋃₁·(var x₂))·(var x₃))))
+
+lemma AxiomS1_univ_of_base : (isBase (axiomS1 x₁ x₂)) := by
+  unfold axiomS1
+  have H1 := b_atom (isAtomic.at_mem (var x₁) (𝔰₁·(var x₂)))
+  have H2 := b_atom (isAtomic.at_eq (var x₁) (var x₂))
+  exact Iff_base (var x₁∈₁𝔰₁·var x₂) (var x₁=₁var x₂) H1 H2
+
+lemma AxiomS2_univ_of_base : (isBase (axiomS2 x₁ x₂ x₃)) := by
+  unfold axiomS2
+  have H1 := b_atom (isAtomic.at_mem (var x₁) ((∪₁·(var x₂))·(var x₃)))
+  have H2 := b_atom (isAtomic.at_mem (var x₁) (var x₂))
+  have H3 := b_atom (isAtomic.at_mem (var x₁) (var x₃))
+  have H4 := b_or H2 H3
+  exact Iff_base (var x₁∈₁(∪₁·var x₂)·var x₃) ((var x₁∈₁var x₂).or (var x₁∈₁var x₃)) H1 H4
+
+lemma AxiomS3_univ_of_base : (isBase (axiomS3 b a f x)) := by
+  unfold axiomS3
+  have H1 := b_atom (isAtomic.at_mem (var b) ((ind_⋃₁·(var a))·(var f)))
+  have H2 := b_atom (isAtomic.at_mem (var b) ((var f)·(var x)))
+  have H3 := bExists_base x (var a) H2
+  exact Iff_base (var b∈₁(ind_⋃₁·var a)·var f) (b∃₁₁ x (var a) (var b∈₁var f·var x)) H1 H3
+
+lemma AxiomS4_univ_of_base : (isBase (axiomS4 x₁ x₂)) := by
+  unfold axiomS4
+  have H := b_atom (isAtomic.at_mem (var x₂) (var x₁))
+  exact bExists_base x₂ (var x₁) H
+
+
+
+
+
+
+
+
+def AxiomE1 (x : String) : Formula :=
+  ∀₁₁ x (axiomE1 x)
+def AxiomE2 (x₁ x₂ : String) (A : Formula) (hA : isBase A) : Formula :=
+  ∀₁₁ x₁ (∀₁₁ x₂ (axiomE2 x₁ x₂ A hA))
+def AxiomUn (x : String) (t : String) (A : Formula) : Formula :=
+  ∀₁₁ t (axiomUn x t A)
+def AxiomC1 (x₁ x₂ : String) : Formula :=
+  ∀₁₁ x₁ (∀₁₁ x₂ (axiomC1 x₁ x₂))
+def AxiomC2 (x₁ x₂ x₃ : String) : Formula :=
+  ∀₁₁ x₁ (∀₁₁ x₂ (∀₁₁ x₃ (axiomC2 x₁ x₂ x₃)))
+def AxiomP1 (x₁ x₂ : String) : Formula :=
+  ∀₁₁ x₁ (∀₁₁ x₂ (axiomP1 x₁ x₂))
+def AxiomP2 (x₁ x₂ x₃ : String) : Formula :=
+  ∀₁₁ x₁ (∀₁₁ x₂ (∀₁₁ x₃ (axiomP2 x₁ x₂ x₃)))
+def AxiomS1 (x₁ x₂ : String) : Formula :=
+  ∀₁₁ x₁ (∀₁₁ x₂ (axiomS1 x₁ x₂))
+def AxiomS2 (x₁ x₂ x₃ : String) : Formula :=
+  ∀₁₁ x₁ (∀₁₁ x₂ (∀₁₁ x₃ (axiomS2 x₁ x₂ x₃)))
+def AxiomS3 (b a f x : String) : Formula :=
+  ∀₁₁ a (∀₁₁ f (∀₁₁ b (axiomS3 b a f x)))
+def AxiomS4 (x₁ x₂ : String) : Formula :=
+  ∀₁₁ x₁ (axiomS4 x₁ x₂)
+
+
+
+
+
+
+
+
+
+
+
+/- PARA COPIAR
+lemma Axiom_univ_of_base : (isBase ()) := by sorry
+-/
+
+
+
+-- Versão mega completa mas com [] o que é chato para as provas
+def BAxiomE1 (x : String) : Formula :=
+  ∀₁ [x]                ((var x)=₁(var x))
+def BAxiomE11 (x : String) : Formula :=
+  ∀₁₁ x                 ((var x)=₁(var x))
+def BAxiomE2 (x₁ x₂ : String) (A : Formula) (hA : isBase A) : Formula :=
+  ∀₁ [x₁,x₂]            ((var x₁)=₁(var x₂)) ∧₁ (A →₁ (A.subst (HashMap.ofList ([x₁].zip ([x₂].tt)))))
+def BAxiomUn (x : String) (t : String) (A : Formula) : Formula :=
+  ∀₁ [t]                (b∀₁₁ x (var t) A) ↔₁ (∀₁₁ x (((var x) ∈₁ (var t)) →₁ A))
+def BAxiomC1 (x₁ x₂ : String) : Formula :=
+  ∀₁ [x₁,x₂]            (((Π₁·(var x₁))·(var x₂)) =₁ (var x₁))
+def BAxiomC2 (x₁ x₂ x₃ : String) : Formula :=
+  ∀₁ [x₁, x₂, x₃]       ((((Σ₁·(var x₁))·(var x₂))·(var x₃)) =₁ (((var x₁)·(var x₃))·((var x₂)·(var x₃))))
+def BAxiomP1 (x₁ x₂ : String) : Formula :=
+  ∀₁ [x₁,x₂]            (((ind_⋃₁·(𝔰₁·(var x₁)))·(var x₂)) =₁ ((var x₂)·(var x₁)))
+def BAxiomP2 (x₁ x₂ x₃ : String) : Formula :=
+  ∀₁ [x₁, x₂, x₃]       (((ind_⋃₁·((∪₁·(var x₁))·(var x₂)))·(var x₃)) =₁ ((∪₁·((ind_⋃₁·(var x₁))·(var x₃)))·((ind_⋃₁·(var x₂))·(var x₃))))
+def BAxiomS1 (x₁ x₂ : String) : Formula :=
+  ∀₁ [x₁,x₂]            (((var x₁) ∈₁ (𝔰₁·(var x₂))) ↔₁ ((var x₁) =₁ (var x₂)))
+def BAxiomS2 (x₁ x₂ x₃ : String) : Formula :=
+  ∀₁ [x₁, x₂, x₃]       ((var x₁) ∈₁ ((∪₁·(var x₂))·(var x₃)) ) ↔₁ (((var x₁) ∈₁ (var x₂)) ∨₁ ((var x₁) ∈₁ (var x₃)))
+def BAxiomS3 (b a f x : String) : Formula :=
+  ∀₁ [a, f, b]          (((var b) ∈₁ ((ind_⋃₁·(var a))·(var f))) ↔₁ (b∃₁₁ x (var a) ((var b) ∈₁ ((var f)·(var x)))))
+def BAxiomS4 (x₁ x₂ : String) : Formula :=
+  ∀₁ [x₁]               (b∃₁₁ x₂ (var x₁) ((var x₂) ∈₁ (var x₁)))
 
 end Axioms
 
+--def Axreflexivity (x : String) : Formula := (Term.var x) =₁ (Term.var x)
 
 
-def Axreflexivity (x : String) : Formula := (Term.var x) =₁ (Term.var x)
+/-
+lemma AxiomE1_univ_of_base (x : String) : (isBase ((var x)=₁(var x))) := by
+  exact b_atom (isAtomic.at_eq (var x) (var x))
+-/
+
 
 
 section
@@ -55,56 +226,54 @@ local infix:27 " ⊢ " => ProvableFrom
 open Axioms
 
 inductive ProvableFrom : Set Formula → Formula → Prop
-| ax    : ∀ {Γ A},   A ∈ Γ   → Γ ⊢ A
-| impI  : ∀ {Γ A B},  insert A Γ ⊢ B                 → Γ ⊢ A →₁ B
-| impE  : ∀ {Γ A B},           Γ ⊢ (A →₁ B) → Γ ⊢ A  → Γ ⊢ B
-| andI  : ∀ {Γ A B},           Γ ⊢ A        → Γ ⊢ B  → Γ ⊢ A ∧₁ B
-| andE1 : ∀ {Γ A B},           Γ ⊢ (A ∧₁ B)          → Γ ⊢ A
-| andE2 : ∀ {Γ A B},           Γ ⊢ (A ∧₁ B)          → Γ ⊢ B
-| orI1  : ∀ {Γ A B},           Γ ⊢ A                → Γ ⊢ (A ∨₁ B)
-| orI2  : ∀ {Γ A B},           Γ ⊢ B                → Γ ⊢ (A ∨₁ B)
-| orE   : ∀ {Γ A B C}, Γ ⊢ (A ∨₁ B) → insert A Γ ⊢ C → insert B Γ ⊢ C → Γ ⊢ C
+| ax    : ∀ {Γ A},            A ∈ Γ             → Γ ⊢ A
 
 -- TWO AXIOM SCHEMA:
-| exMid : ∀ {A},               ∅ ⊢ ((¬₁A)∨₁A)
---| subs : ∀ {A},              ∅ ⊢ ((∀₁ x A) →₁ A)     -- TBD: falta substituição aqui
+| exMid : ∀ {A},              Γ ⊢ ((¬₁A)∨₁A)
+| subs : ∀ {A},               Γ ⊢ ((∀₁ x A) →₁ (A.subst (HashMap.ofList (x.zip t))))
 
 -- FIVE RULES:
-| exp :     ∀ {A B},          ∅ ⊢ A             →   ∅ ⊢ (B∨₁A)
-| contrad : ∀ {A},            ∅ ⊢ (A∨₁A)        →   ∅ ⊢ A
-| assoc :   ∀ {A B C},        ∅ ⊢ (A∨₁(B∨₁C))   →   ∅ ⊢ ((A∨₁B)∨₁C)
-| cut :     ∀ {A B C},        ∅ ⊢ (A∨₁B)        →   ∅ ⊢ ((¬₁A)∨₁C)    →   ∅ ⊢ (B∨₁C)
---| forallInt : ∀ {A B},      ∅ ⊢ (A∨₁B)    →   ∅ ⊢ ((∀₁ x A)∨₁B)   -- TBD: falta substituição aqui
+| exp :     ∀ {A B},          Γ ⊢ A             →   Γ ⊢ (B∨₁A)
+| contrad : ∀ {A},            Γ ⊢ (A∨₁A)        →   Γ ⊢ A
+| assoc :   ∀ {A B C},        Γ ⊢ (A∨₁(B∨₁C))   →   Γ ⊢ ((A∨₁B)∨₁C)
+| cut :     ∀ {A B C},        Γ ⊢ (A∨₁B)        →   Γ ⊢ ((¬₁A)∨₁C)      →   Γ ⊢ (B∨₁C)
+| forallInt : ∀ {A B},        Γ ⊢ (A∨₁B)        →   Γ ⊢ ((∀₁ x A)∨₁B)   -- TBD: falta x does not occur free in B
 
 -- AXIOMS:
-| AxE₁ (t:Term) :                               ∅ ⊢ (t=₁t)
-| AxE₂ (t₁ t₂ :Term) (hA : isBase A) :          ∅ ⊢ ((t₁=₁t₂) ∧₁ (A →₁ A))     -- TBD: falta substituição aqui
-| AxU (x : String) (t : Term) (A : Formula) :   ∅ ⊢ ((b∀₁₁ x t A) ↔₁ (∀₁₁ x (((var x) ∈₁ t) →₁ A)))
-| AxC₁ (t₁ t₂ : Term) :                         ∅ ⊢ (((Π₁·t₁)·t₂) =₁ t₁)
-| AxC₂ (t₁ t₂ t₃ : Term) :                      ∅ ⊢ ((((Σ₁·t₁)·t₂)·t₃) =₁ ((t₁·t₃)·(t₂·t₃)))
-| AxP₁ (t₁ t₂ : Term) :                         ∅ ⊢ (((ind_⋃₁·(𝔰₁·t₁))·t₂) =₁ (t₂·t₁))
-| AxP₂ (t₁ t₂ t₃ : Term) :                      ∅ ⊢ (((ind_⋃₁·((∪₁·t₁)·t₂))·t₃) =₁ ((∪₁·((ind_⋃₁·t₁)·t₃))·((ind_⋃₁·t₂)·t₃)))
-| AxS₁ (t₁ t₂ : Term) :                         ∅ ⊢ ((t₁ ∈₁ (𝔰₁·t₂)) ↔₁ (t₁ =₁ t₂))
-| AxS₂ (t₁ t₂ t₃ : Term) :                      ∅ ⊢ ((t₁ ∈₁ ((∪₁·t₂)·t₃) ) ↔₁ ((t₁ ∈₁ t₂) ∨₁ (t₁ ∈₁ t₃)))
-| AxS₃ (a f b : Term) :                         ∅ ⊢ ((b ∈₁ ((ind_⋃₁·a)·f)) ↔₁ (b∃₁₁ x a (b ∈₁ (f·(var x)))))
+| AxE₁:                       Γ ⊢ AxiomE1 x
+| AxE₂:                       Γ ⊢ AxiomE2 x₁ x₂ A hA
+| AxU:                        Γ ⊢ AxiomUn x t A
+| AxC₁:                       Γ ⊢ AxiomC1 x₁ x₂
+| AxC₂:                       Γ ⊢ AxiomC2 x₁ x₂ x₃
+| AxP₁:                       Γ ⊢ AxiomP1 x₁ x₂
+| AxP₂:                       Γ ⊢ AxiomP2 x₁ x₂ x₃
+| AxS₁:                       Γ ⊢ AxiomS1 x₁ x₂
+| AxS₂:                       Γ ⊢ AxiomS2 x₁ x₂ x₃
+| AxS₃:                       Γ ⊢ AxiomS3 a f b x
+| AxS₄:                       Γ ⊢ AxiomS4 x₁ x₂
+
+-- ax, exMid, subs, exp, contrad, assoc, cut, forallInt, AxE₁, AxE₂, AxU, AxC₁, AxC₂, AxP₁, AxP₂, AxS₁, AxS₂, AxS₃, AxS₄
+
+/-
+| AxE₁ (t:Term) :                               Γ ⊢ (t=₁t)
+| AxE₂ (t₁ t₂ :Term) (hA : isBase A) :          Γ ⊢ ((t₁=₁t₂) ∧₁ (A →₁ A))     -- TBD: falta substituição aqui
+| AxU (x : String) (t : Term) (A : Formula) :   Γ ⊢ ((b∀₁₁ x t A) ↔₁ (∀₁₁ x (((var x) ∈₁ t) →₁ A)))
+| AxC₁ (t₁ t₂ : Term) :                         Γ ⊢ (((Π₁·t₁)·t₂) =₁ t₁)
+| AxC₂ (t₁ t₂ t₃ : Term) :                      Γ ⊢ ((((Σ₁·t₁)·t₂)·t₃) =₁ ((t₁·t₃)·(t₂·t₃)))
+| AxP₁ (t₁ t₂ : Term) :                         Γ ⊢ (((ind_⋃₁·(𝔰₁·t₁))·t₂) =₁ (t₂·t₁))
+| AxP₂ (t₁ t₂ t₃ : Term) :                      Γ ⊢ (((ind_⋃₁·((∪₁·t₁)·t₂))·t₃) =₁ ((∪₁·((ind_⋃₁·t₁)·t₃))·((ind_⋃₁·t₂)·t₃)))
+| AxS₁ (t₁ t₂ : Term) :                         Γ ⊢ ((t₁ ∈₁ (𝔰₁·t₂)) ↔₁ (t₁ =₁ t₂))
+| AxS₂ (t₁ t₂ t₃ : Term) :                      Γ ⊢ ((t₁ ∈₁ ((∪₁·t₂)·t₃) ) ↔₁ ((t₁ ∈₁ t₂) ∨₁ (t₁ ∈₁ t₃)))
+| AxS₃ (a f b : Term) :                         Γ ⊢ ((b ∈₁ ((ind_⋃₁·a)·f)) ↔₁ (b∃₁₁ x a (b ∈₁ (f·(var x)))))
 -- TBD: FALTA AXS4
-| AxE1 (t:Term):          ∅ ⊢ AxiomE1 t
-| AxE2:          ∅ ⊢ AxiomE2 t₁ t₂ A hA
-| AxUu:          ∅ ⊢ AxiomU x t A
-| AxC1:          ∅ ⊢ AxiomC1 t₁ t₂
-| AxC2:          ∅ ⊢ AxiomC2 t₁ t₂ t₃
-| AxP1:          ∅ ⊢ AxiomP1 t₁ t₂
-| AxP2:          ∅ ⊢ AxiomP2 t₁ t₂ t₃
-| AxS1:          ∅ ⊢ AxiomS1 t₁ t₂
-| AxS2:          ∅ ⊢ AxiomS2 t₁ t₂ t₃
-| AxS3:          ∅ ⊢ AxiomS3 a f b x
--- TBD: FALTA AXS4
+-/
 
 end
 
-def bAC (x y f : String) (A : Formula) : Formula := (∀₁₁ x (∃₁₁ y A)) →₁ (∃₁₁ f (∀₁₁ x (b∃₁₁ y ((Term.var f)·(Term.var x)) A)))     -- bAC^ω_*
+def bAC (x y f : List String) (A : Formula) : Formula := (∀₁ x (∃₁ y A)) →₁ (∃₁ f (∀₁ x (bExistsTuple2 y ((f.tt)⊙(x.tt)) A)))     -- bAC^ω_*
 
-local infix:27 (priority := high) " ⊢ " => ProvableFrom     -- já não é a mesma notação que em ProvableFrom!
+
+infix:27 (priority := high) " ⊢ " => ProvableFrom     -- já não é a mesma notação que em ProvableFrom!
 
 /- A formula is provable if there is a -/
 /-
@@ -117,7 +286,7 @@ without relying on any specific assumptions.
 -- DEF: A formula is said to be provable if it can be derived using ProvableFrom and nothing else
 def Provable (A : Formula) := ∅ ⊢ A
 
-export ProvableFrom (ax impI impE andI andE1 andE2 orI1 orI2 orE)
+export ProvableFrom (ax exMid subs exp contrad assoc cut forallInt AxE₁ AxE₂ AxU AxC₁ AxC₂ AxP₁ AxP₂ AxS₁ AxS₂ AxS₃ AxS₄)
 variable {Γ Δ : Set Formula}
 
 /- We define a simple tactic `apply_ax` to prove something using the `ax` rule. -/
@@ -146,16 +315,12 @@ theorem term_reflexivity {t:Term}: ∅ ⊢ (t =₁ t) :=
 -/
 
 example (A : Formula) : (insert (bAC x y f B) ∅ ⊢ A) → (Provable A) := by sorry
-theorem Soundness (A : Formula) : (insert (bAC x y f B) ∅ ⊢ A) → (∃(t:Term), (Provable (∀₁ a A))) := by sorry    -- TBD: falta subst aqui
+theorem Soundness (A : Formula) : (insert (bAC x y f B) ∅ ⊢ A) → (∃(t: List Term), (Provable (∀₁ a A))) := by sorry    -- TBD: falta subst aqui
 theorem Characterization (A : Formula) : (insert (bAC x y f B) ∅ ⊢ A) → (Provable (A ∨₁ A)) := by sorry          -- TBD: falta A^SH aqui
-lemma Lem32 (A : Formula) (hA : isBase A) : (insert (bAC x y f B) ∅ ⊢ ((b∀₁₁ x t (∃₁₁ y A)) →₁ (∃₁₁ b (b∀₁₁ x t (b∃₁₁ y (var b) A))))) := by sorry
+lemma Lem32 (A : Formula) (hA : isBase A) : (insert (bAC x y f B) ∅ ⊢ ((b∀₁ x t (∃₁ y A)) →₁ (∃₁ b (b∀₁ x t (bExistsTuple2 y (b.tt) A))))) := by sorry
 
 
-example : insert A (insert B ∅) ⊢ A ∧₁ B := by
-  exact andI (ax (mem_insert _ _)) (ax (mem_insert_of_mem _ (mem_insert _ _)))
 
-example : insert A (insert B ∅) ⊢ A ∧₁ B := by
-  exact andI (by apply_ax) (by apply_ax)
 
 /-
 example : insert A (insert B ∅) ⊢ A ∧₁ B := by
